src/SerialFacts.v
@@ -4,21 +4,9 @@ Require Import Syntax Semantics SemFacts StepDet Serial.
 
 Set Implicit Arguments.
 
-Lemma atomic_nil_in:
-  forall sys min mouts,
-    Atomic sys min nil mouts ->
-    forall msg,
-      In msg mouts ->
-      msg = min.
-Proof.
-  intros; inv H.
-  Common.dest_in.
-  reflexivity.
-Qed.
-
 Lemma atomic_emptyILabel_not_in:
-  forall sys min hst mouts,
-    Atomic sys min hst mouts ->
+  forall sys tid min hst mouts,
+    Atomic sys tid min hst mouts ->
     ~ In emptyILabel hst.
 Proof.
   induction 1; simpl; intros; [auto|].
@@ -28,8 +16,8 @@ Proof.
 Qed.
 
 Lemma atomic_iLblIn_not_in:
-  forall sys min hst mouts,
-    Atomic sys min hst mouts ->
+  forall sys tid min hst mouts,
+    Atomic sys tid min hst mouts ->
     forall msg,
       ~ In (IlblIn msg) hst.
 Proof.
@@ -40,16 +28,16 @@ Proof.
 Qed.
 
 Lemma atomic_preserved:
-  forall impl1 min hst mouts,
-    Atomic impl1 min hst mouts ->
+  forall impl1 tid min hst mouts,
+    Atomic impl1 tid min hst mouts ->
     forall impl2,
       indicesOf impl1 = indicesOf impl2 ->
-      Atomic impl2 min hst mouts.
+      Atomic impl2 tid min hst mouts.
 Proof.
   induction 1; simpl; intros.
   - constructor; auto.
     unfold isExternal in *.
-    rewrite H0 in H; assumption.
+    rewrite H1 in H; assumption.
   - constructor; auto.
 Qed.
 
